src/theories/machine_base.v
@@ -1,0 +1,214 @@
+From stdpp Require Import countable fin.
+From Coq Require Import ssreflect Bool Eqdep_dec.
+From ExtLib Require Import Structures.Monads.
+
+Open Scope general_if_scope.
+
+(* TODO: ZArith seems to be much more convenient *)
+(*
+Class MachineParameters := {
+  WordUpperBound : nat;
+  WordHasAtLeastTwoValues : 1 < WordUpperBound;
+  RegCountUpperBound : nat;
+  RegCountAtLeastOne : 0 < RegCountUpperBound;
+  AddressSpaceSize : nat;
+                          }.
+
+Context `(MachineParams : MachineParameters).
+ *)
+
+Definition WordUpperBound := 65536.
+Definition RegCountUpperBound := 32.
+Definition AddressSpaceSize := 512.
+
+Definition Word : Type :=
+  fin WordUpperBound.
+
+Instance eqDecisionWord : EqDecision Word.
+Proof.
+  solve_decision.
+Qed.
+
+Instance countableWord : Countable Word.
+Proof.
+  refine {| encode := _;
+            decode := _;
+            decode_encode := _ |}.
+  apply fin_countable.
+Qed.
+
+Inductive RegName : Type :=
+| PC
+| NZ
+| R (n : nat) (fin : n < RegCountUpperBound).
+
+Instance eqDecisionRegName : EqDecision RegName.
+Proof.
+  intros x y. destruct x as [| | n fin], y as [| | n' fin']; try (by left); try (by right).
+  destruct (nat_eq_dec n n').
+  - subst n'; left; f_equal; apply proof_irrel.
+  - right; congruence.
+Qed.
+
+Program Definition n_to_regname (n : nat) : option RegName :=
+  if (nat_lt_dec n RegCountUpperBound) then Some (R n _) else None.
+Next Obligation.
+  auto.
+Defined.
+
+Instance countableRegName : Countable RegName.
+Proof.
+  refine {| encode r := encode match r with
+                               | PC => inl false
+                               | NZ => inl true
+                               | R n fin => inr n
+                               end;
+            decode n := match (decode n) with
+                        | Some (inl false) => Some PC
+                        | Some (inl true) => Some NZ
+                        | Some (inr n) => n_to_regname n
+                        | None => None
+                        end;
+            decode_encode := _ |}.
+  intro r. destruct r; auto.
+  rewrite decode_encode.
+  unfold n_to_regname.
+  destruct (nat_lt_dec n RegCountUpperBound).
+  - do 2 f_equal; apply proof_irrel.
+  - exfalso; auto.
+Qed.
+
+Inductive Ownership : Type :=
+| Owned
+| NotOwned.
+
+Instance eqDecisionOwnership : EqDecision Ownership.
+Proof.
+  solve_decision.
+Qed.
+
+Inductive Access : Type :=
+| NoAccess
+| SharedAccess
+| ExclusiveAccess.
+
+Instance eqDecisionAccess : EqDecision Access.
+Proof.
+  solve_decision.
+Qed.
+
+Definition Perm : Type :=
+  (Ownership * Access).
+
+Definition isAccessible (p : Perm) : bool :=
+  match p with
+  | (_, SharedAccess) => true
+  | (_, ExclusiveAccess) => true
+  | _ => false
+  end.
+
+Definition isOwned (p : Perm) : bool :=
+  match p with
+  | (Owned, _) => true
+  | _ => false
+  end.
+
+Instance eqDecisionPerm : EqDecision Perm.
+Proof.
+  solve_decision.
+Qed.
+
+Inductive TransactionType : Type :=
+| Donation
+| Sharing
+| Lending.
+
+Instance eqDecisionTransactionType : EqDecision TransactionType.
+Proof.
+  solve_decision.
+Qed.
+
+Inductive Instruction : Type :=
+| Mov (dst : RegName) (src : Word + RegName)
+| Ldr (dst : RegName) (src : RegName)
+| Str (src : RegName) (dst : RegName)
+| Cmp (arg1 : RegName) (arg2 : Word + RegName)
+| Jnz (arg : RegName)
+| Jmp (arg : RegName)
+| Halt
+| Fail
+| Hvc.
+
+Class InstructionSerialization := {
+  DecodeInstr : Word -> option Instruction;
+  EncodeInstr : Instruction -> Word;
+  DecodeEncodeInstr : forall (i : Instruction), DecodeInstr (EncodeInstr i) = Some i;
+                                 }.
+
+Context `(InstrSer : InstructionSerialization).
+
+Instance eqDecisionInstruction : EqDecision Instruction.
+Proof.
+  solve_decision.
+Qed.
+
+Instance countableInstruction : Countable Instruction.
+Proof.
+  refine {| encode := fun i => encode (EncodeInstr i);
+            decode := fun p => match decode p with
+                               | None => None
+                               | Some p' => DecodeInstr p'
+                               end;
+            decode_encode := _ |}.
+  intros x.
+  rewrite decode_encode.
+  apply DecodeEncodeInstr.
+Qed.
+
+Definition Addr : Type :=
+  fin AddressSpaceSize.
+
+Instance eqDecisionAddr : EqDecision Addr.
+Proof.
+  solve_decision.
+Qed.
+
+Instance countableAddr : Countable Addr.
+Proof.
+  refine {| encode := _;
+            decode := _;
+            decode_encode := _ |}.
+  apply fin_countable.
+Qed.
+
+Inductive HvcFunc : Type :=
+  Run
+| Yield
+| Share
+| Lend 
+| Donate
+| Retrieve
+| Relinquish
+| Reclaim
+| Send 
+| Receive
+| Wait.
+
+Inductive HvcError : Type :=
+  InvParam
+| Denied
+| Busy
+| Ready.
+
+Class HypervisorParameters := {
+  VMCount : nat;
+  VMCountPos : 0 < VMCount;
+  DecodeVMID : Word -> option (fin VMCount);
+  EncodeVMID : (fin VMCount)  -> Word;
+  DecodeEncodeVMID : forall (vmid : fin VMCount),
+      DecodeVMID (EncodeVMID vmid) = Some vmid;
+  DecodeHvcFunc : Word -> option HvcFunc;
+  EncodeHvcFunc : HvcFunc -> Word;
+  DecodeEncodeHvcFunc : forall (hvc : HvcFunc),
+      DecodeHvcFunc (EncodeHvcFunc hvc) = Some hvc;
+                             }.
